src/RsUpRed.v
@@ -1,0 +1,61 @@
+Require Import Peano_dec Omega List ListSupport.
+Require Import Common FMap.
+Require Import Syntax Semantics SemFacts StepM Invariant.
+Require Import Serial SerialFacts.
+Require Import Reduction Commutativity QuasiSeq Topology.
+Require Import RqRsTopo RqRsFacts.
+Require Import RqRsInvMsg RqRsInvLock RqRsInvAtomic.
+
+Set Implicit Arguments.
+
+Open Scope list.
+Open Scope fmap.
+
+Section RsUpReduction.
+  Context {oifc: OStateIfc}.
+  Variables (dtr: DTree)
+            (sys: System oifc).
+
+  Hypothesis (Hrrs: RqRsSys dtr sys).
+
+  Ltac disc_rule_custom ::=
+    try disc_footprints_ok.
+
+  Lemma rsUp_lbl_reducible:
+    forall dtr oidxTo rsUps,
+      RsUpMsgs dtr oidxTo rsUps ->
+      forall oidx1 ridx1 rins1 routs1 oidx2 ridx2 routs2,
+        DisjList rsUps rins1 ->
+        Reducible
+          sys [RlblInt oidx2 ridx2 rsUps routs2;
+                 RlblInt oidx1 ridx1 rins1 routs1]
+          [RlblInt oidx1 ridx1 rins1 routs1;
+             RlblInt oidx2 ridx2 rsUps routs2].
+  Proof.
+  Admitted.
+
+  Lemma rsUp_rpush_unit_ok_ind:
+    forall oidxTo rsUps inits ins hst outs eouts
+           oidx ridx routs,
+      RsUpMsgs dtr oidxTo rsUps ->
+      Atomic msg_dec inits ins hst outs eouts ->
+      DisjList rsUps inits ->
+      Reducible sys (RlblInt oidx ridx rsUps routs :: hst)
+                (hst ++ [RlblInt oidx ridx rsUps routs]).
+  Proof.
+    induction 2; simpl; intros; subst.
+    - eapply rsUp_lbl_reducible; eauto.
+    - eapply reducible_trans.
+      + apply reducible_cons_2.
+        eapply rsUp_lbl_reducible.
+        * eassumption.
+        * eapply DisjList_comm, DisjList_SubList; [eassumption|].
+          admit.
+      + apply reducible_cons; auto.
+  Admitted.
+  
+End RsUpReduction.
+
+Close Scope list.
+Close Scope fmap.
+
